Include documentation

Encoding_Nat.thy
@@ -2,22 +2,43 @@
   Author: Maximilian Spitz
 *)
 
-theory Encoding_Nat imports Main begin
+
+section \<open>An Encoding for Natural Numbers\<close>
+
+theory Encoding_Nat
+  imports Main
+begin
+
+text \<open>
+At first, an encoding of naturals as lists of digits with respect to
+  an arbitrary base $b \geq 2$ is introduced,
+  because the presented Gray code and its properties
+  are reasonably expressed in terms of a word representation of numbers.
+\<close>
 
 
-section \<open>Valuation and Validity\<close>
+subsection \<open>Validity and Valuation\<close>
 
-type_synonym BASE = nat
+text \<open>
+In the context of a given base not all possible code words are valid
+  number representations.
+A validity predicate is defined, that checks if a code word is valid
+  and a valuation to obtain the number represented by a valid word.
+\<close>
+
+type_synonym base = nat
 
 type_synonym word = "nat list"
 
-fun val :: "BASE \<Rightarrow> word \<Rightarrow> nat" where
+fun val :: "base \<Rightarrow> word \<Rightarrow> nat" where
   "val b [] = 0"
 | "val b (a#w) = a + b*val b w"
 
-fun valid :: "BASE \<Rightarrow> word \<Rightarrow> bool" where
+fun valid :: "base \<Rightarrow> word \<Rightarrow> bool" where
   "valid b [] \<longleftrightarrow> 2\<le>b"
 | "valid b (a#w) \<longleftrightarrow> a<b \<and> valid b w"
+
+text \<open>Given a base, the value of a valid word is bound by its length.\<close>
 
 lemma val_bound:
   "valid b w \<Longrightarrow> val b w < b^length(w)"
@@ -37,24 +58,40 @@ lemma valid_base:
   by (induction w) auto
 
 
-section \<open>Encoding Numbers as Words\<close>
+subsection \<open>Encoding Numbers as Words\<close>
 
-fun enc :: "BASE \<Rightarrow> nat \<Rightarrow> word" where
+text \<open>
+It was stated that not all code words are valid. Similarly, numbers do not
+  have a unique word representation in general.
+Therefore, it is reasonable to normalise representations with respect
+  to either value or word length.
+A normal representation w.r.t. value is without leading zeroes.
+However, if the word length is fixed, numbers can be represented
+  only up to an upper bound. Note that this bound is stated above.
+\<close>
+
+fun enc :: "base \<Rightarrow> nat \<Rightarrow> word" where
   "enc _ 0 = []"
 | "enc b n = (if 2\<le>b then n mod b#enc b (n div b) else undefined)"
 
-fun enc_len :: "BASE \<Rightarrow> nat \<Rightarrow> nat" where
+fun enc_len :: "base \<Rightarrow> nat \<Rightarrow> nat" where
   "enc_len _ 0 = 0"
 | "enc_len b n = (if 2\<le>b then Suc(enc_len b (n div b)) else undefined)"
 
-fun lenc :: "nat \<Rightarrow> BASE \<Rightarrow> nat \<Rightarrow> word" where
+fun lenc :: "nat \<Rightarrow> base \<Rightarrow> nat \<Rightarrow> word" where
   "lenc 0 _ _ = []"
 | "lenc (Suc k) b n = n mod b#lenc k b (n div b)"
 
-definition normal :: "BASE \<Rightarrow> word \<Rightarrow> bool" where
+definition normal :: "base \<Rightarrow> word \<Rightarrow> bool" where
   "normal b w \<equiv> enc_len b (val b w) = length w"
 
-section \<open>Correctness\<close>
+
+subsection \<open>Correctness\<close>
+
+text \<open>
+Now, the expected properties of above definitions are proven as well as
+  that they interact correctly.
+\<close>
 
 lemma length_enc:
   "2\<le>b \<Longrightarrow> length (enc b n) = enc_len b n"
@@ -165,12 +202,24 @@ theorem enc_correct:
   "2\<le>b \<Longrightarrow> bij_betw (enc b) UNIV {w. valid b w \<and> normal b w}"
   by (simp add: bij_betw_def inj_enc range_enc)
 
+text \<open>
+Given a valid base $b$ and length $k$, we encode exactly the first $b^k$ numbers.
+\<close>
+
 theorem lenc_correct:
   "2\<le>b \<Longrightarrow> bij_betw (lenc k b) {..<b^k} {w. valid b w \<and> length w = k}"
   by (simp add: bij_betw_def inj_lenc range_lenc)
 
 
-section \<open>Circular Increment Operation\<close>
+subsection \<open>Circular Increment Operation\<close>
+
+text \<open>
+It is beneficial for our purpose to have an increment operation on
+  words of fixed length that wraps around.
+Mathematically, this corresponds to adding 1 in the additive group
+  of the factor ring of the integers modulo ($b^k$).
+Correctness is proven in terms of previously verified operations.
+\<close>
 
 fun inc :: "nat \<Rightarrow> word \<Rightarrow> word" where
   "inc _ [] = []"
@@ -184,7 +233,13 @@ lemma valid_inc:
   "valid b w \<Longrightarrow> valid b (inc b w)"
   by (induction w) auto
 
-lemma val_inc:
+text \<open>
+Note that the following fact shows that we do not only have an encoding
+  in the sense that it is a bijection but we also preserve a certain structure,
+  that is necessary for the purpose of reasoning about Gray codes.
+\<close>
+
+theorem val_inc:
   "valid b w \<Longrightarrow> val b (inc b w) = Suc (val b w) mod b^length(w)"
 proof (induction w)
   case Nil thus ?case by simp
